# 定理 1

[toc]

## 定理

对于给定的实矩阵$\Upsilon_{1} \leq 0$, $\Upsilon_{2}, \Upsilon_{3} > 0$, 和 $\Upsilon_{4} \geq 0$，满足$(\|\Upsilon_{1}\| + \|\Upsilon_{2}\|)\cdot \|\Upsilon_{4}\| = 0$，以及标量 $\varepsilon_{1}, \varepsilon_{2}, \gamma > 0, \delta \geq 0, d > 0, \alpha > 0, \sigma \geq 0$。

假设对于任意 $i \in \bar{\mathbb{N}}$，存在矩阵$P_i > 0$, $U > 0$,$\bar{Q} = \begin{bmatrix} Q_1 & Q_2 \\ * & Q_3 \end{bmatrix} > 0$,$Y$, $H_m$ $(m = 1,2,3,4,5)$, $G_n$ $(n = 1,2,3,4)$，以及矩阵 $\Lambda_i \geq 0$，使得
$$\begin{aligned}&\Psi(i)=\begin{bmatrix}\Psi_{11}(i)&\Psi_{12}(i)&\Psi_{13}(i)&\Psi_{14}&\Psi_{15}(i)&\Psi_{16}\\*&\Psi_{22}&\Psi_{23}(i)&0&\Psi_{25}(i)&\Psi_{26}\\*&*&\Psi_{33}(i)&\Psi_{34}&\Psi_{35}(i)&\Psi_{36}\\*&*&*&\Psi_{44}&0&\Psi_{46}\\*&*&*&*&\Psi_{55}&0\\*&*&*&*&*&\Psi_{66}\end{bmatrix}<0,\\&\Theta(i)=\begin{bmatrix}\Theta_{11}(i)&\Theta_{12}(i)&\Theta_{13}(i)&\Theta_{14}&\Theta_{15}(i)\\*&\Theta_{22}&\Theta_{23}(i)&\Theta_{24}&\Theta_{25}(i)\\*&*&\Theta_{33}(i)&\Theta_{34}&\Theta_{35}(i)\\*&*&*&\Theta_{44}&0\\*&*&*&*&\Theta_{55}\end{bmatrix}<0,\\&\Phi(i)=\begin{bmatrix}\Phi_{11}(i)&\Phi_{12}(i)&\Phi_{13}(i)&\Phi_{14}(i)\\*&\Phi_{22}&\Phi_{23}(i)&\Phi_{24}(i)\\*&*&\Phi_{33}(i)&0\\*&*&*&\Phi_{44}\end{bmatrix}<0,\end{aligned}$$
$$\begin{aligned}&\Xi(i)=\begin{bmatrix}P_i+dS(\frac{H_1}{2})-\Upsilon_4&-dH_1+dH_2&dH_3\\*&-dS(H_2-\frac{H_1}{2})&dH_4\\*&*&dS(\frac{H_5}{2})\end{bmatrix}>0,\\&P_i-\Upsilon_4>0\end{aligned}$$
其中：
$$\begin{aligned}\Psi_{11}(i)&=\sum_{j=1}^N\lambda_{ij}^*P_j+2\alpha P_i+S\left(-\frac{H_1}{2}+G_1+Y\overline{A}_i\right)-Y_1,\\\Psi_{12}(i)&=P_i+G_2-Y+\varepsilon_1\overline{A}_i^TY^T,\\\Psi_{13}(i)&=H_1-H_2+G_3-G_1^T+YB_iK_i+\varepsilon_2\overline{A}_i^TY^T,\\\Psi_{14}&=-H_3+G_4,\Psi_{15}(i)=YC_i-Y_2,\\\Psi_{16}&=\sqrt{d}G_1^T,\Psi_{22}=-\mathcal{S}(\varepsilon_1Y),\\\Psi_{23}(i)&=-G_2^T-\varepsilon_2Y^T+\varepsilon_1YB_iK_i,\\\Psi_{25}(i)&=\varepsilon_1YC_i,\Psi_{26}=\sqrt{d}G_2^T,\\\Psi_{33}(i)&=S\left(H_2-\frac{H_1}{2}-G_3+\varepsilon_2YB_iK_i\right)-de^{-2\alpha d}Q_3,\\\Psi_{34}&=-H_4-e^{-2\alpha d}Q_2^T-G_4,\Psi_{35}(i)=\varepsilon_2YC_i,\Psi_{36}=\sqrt{d}G_3^T,\\\Psi_{44}&=-S\left(\frac{H_5}{2}\right)-\frac{e^{-2\alpha d}}{d}Q_1,\Psi_{46}=\sqrt{d}G_4^T,\\\Psi_{55}&=-\mathrm{Y}_3,\Psi_{66}=-e^{-2\alpha d}U,\\\Phi_{11}(i)&=\sum_{\nu=1,j}^N\lambda_{ij}^*P_j+2\alpha P_i+\sigma\Lambda_i+\mathcal{S}\left(Y\overline{A}_i+YB_iK\right)-\mathcal{Y}_1,\\\Phi_{12}(i)&=P_i-Y+\varepsilon_1\overline{A}_i^TY^T+(\varepsilon_1YB_iK_i)^T,\\\Phi_{13}(i)&=YB_iK_i,\Phi_{14}(i)=YC_i-Y_2,\\\Phi_{22}&=\mathcal{S}(-\varepsilon_1Y),\Phi_{23}(i)=\varepsilon_1YB_iK_i,\Phi_{24}(i)=\varepsilon_1YC_i,\\\Phi_{33}(i)&=-\Lambda_i,\Phi_{44}=\delta I-\mathrm{Y}_3,\\\Theta_{11}(i)&=\Psi_{11}(i)+\alpha dS(H_1)+dS(H_3)+dQ_1-Y_1,\\\Theta_{12}(i)&=\Psi_{12}(i)+d\frac{\mathcal{S}(H_1)}{2},\\\Theta_{13}(i)&=\Psi_{13}(i)+2\alpha d(H_2-H_1)+dH_4^T+dQ_2,\end{aligned}$$

## 证明
